src/FrameStack/SubstSemanticsLabeledLemmas.v
@@ -357,7 +357,7 @@ Qed.
 Lemma params_eval_create :
   forall vals ident vl Fs (v : Val) r eff',
   Forall (fun v => VALCLOSED v) vals ->
-  Some (r, eff') = create_result ident (vl ++ v :: vals) -> (* TODO: side effects *)
+  Some (r, eff') = create_result ident (vl ++ v :: vals) ->
   ⟨ FParams ident vl (map VVal vals) :: Fs, RValSeq [v]⟩ -[1 + 2 * length vals, match eff' with
               | None => []
               | Some x => [x]
@@ -375,3 +375,1115 @@ Proof.
             (1 + 2*length vals) by lia. eapply IHvals; eauto.
     reflexivity. reflexivity.
 Qed.
+
+(**
+*)
+
+From CoreErlang.FrameStack Require Export
+  LabeledTermination.
+
+Lemma terminates_in_k_step :
+  forall fs e fs' e' k sl l, ⟨ fs, e ⟩ -⌊ l ⌋->ₗ ⟨ fs', e' ⟩ ->
+  | fs', e' | sl – k ↓ ->
+  | fs, e | (option_cons l sl) – S k ↓.
+Proof.
+  intros fs e fs' e' k sl l H. induction H.
+  all: econstructor; eassumption.
+Qed.
+
+Theorem semantic_iff_termination :
+  forall k e fs l, terminates_in_k_l_sem fs e k l <-> | fs, e | l – k ↓.
+Proof.
+  split.
+  {
+    revert e fs l. induction k; intros e fs l H.
+    * destruct H as [res [Hres HD]].
+      inversion HD; subst. now constructor.
+    * destruct H as [res [Hres HD]].
+      inversion HD; subst.
+      assert (terminates_in_k_l_sem fs' e' k l0). {
+        eexists. split; eassumption.
+      }
+      unfold terminates_in_k_l_sem in H.
+      apply IHk in H.
+      eapply terminates_in_k_step.
+      apply H0. apply H.
+  }
+  {
+    intros. induction H.
+    all: try destruct IHterminates_in_k as [res0 [Hres0 HD]].
+    all: try (now eexists; split;
+                  [eassumption | econstructor;
+                      [now constructor | eassumption | reflexivity]]).
+    * eexists. split.
+      - eassumption.
+      - econstructor. econstructor; try eassumption.
+        eassumption.
+        destruct l; reflexivity.
+    * eexists. split.
+      - exact Hres0.
+      - econstructor. econstructor; eassumption.
+        eassumption.
+        destruct l; reflexivity.
+    * eexists. split.
+      - eassumption.
+      - econstructor. constructor; eassumption.
+        eassumption.
+        reflexivity.
+    * eexists. split.
+      - eassumption.
+      - econstructor. constructor; eassumption.
+        eassumption.
+        reflexivity.
+    * eexists. split.
+      - eassumption.
+      - constructor.
+  }
+Qed.
+
+(* option tail function *)
+Definition option_tail {A} (l : option A) (sl : list A) 
+  : list A :=
+  match l with
+  | Some s => tail sl
+  | None => sl
+  end.
+
+Theorem terminates_step :
+  forall n fs e l, | fs, e | l – n ↓ -> forall fs' e' l', ⟨fs, e⟩ -⌊l'⌋->ₗ ⟨fs', e'⟩
+->
+  | fs', e' | (option_tail l' l) – n - 1↓.
+Proof.
+  intros. apply semantic_iff_termination in H. destruct H. destruct n.
+  * destruct H. inv H.
+    - subst. inversion H1; subst. inversion H0.
+    - subst. inversion H1; subst. inversion H0.
+  * destruct H.
+    inv H1. apply (step_determinism H0) in H3.
+    inv H3. inv H2.
+    assert (exists y, is_result y /\ ⟨ fs', e' ⟩ -[ n , l0 ]->ₗ ⟨ [], y ⟩). { 
+      eexists. eauto. }
+    apply ex_intro in H4. apply semantic_iff_termination in H1.
+    destruct s; simpl; rewrite Nat.sub_0_r; assumption.
+Qed.
+
+Corollary term_step_term :
+  forall k n fs e l1 l2, | fs, e | l1 ++ l2 – n ↓ 
+  -> forall fs' e' , ⟨fs, e⟩ -[k , l1]->ₗ ⟨fs', e'⟩
+->
+  | fs', e' | l2 – n - k ↓.
+Proof.
+  induction k; intros; inversion H0; subst; auto.
+  * rewrite Nat.sub_0_r. auto.
+  * replace (n - S k) with ((n - 1) - k) by lia. destruct s.
+    - eapply terminates_step with (n := n) (l' := Some s) in H2.
+      2: exact H.
+      eapply IHk in H3. exact H3. exact H2.
+    - eapply terminates_step with (n := n) (l' := None) in H2.
+      2: exact H.
+      eapply IHk in H3. exact H3. exact H2.
+Qed.
+
+Corollary term_step_term_2 :
+  forall k n fs e l l1, | fs, e | l – n ↓ 
+  -> forall fs' e' , ⟨fs, e⟩ -[k , l1]->ₗ ⟨fs', e'⟩
+->
+  | fs', e' | skipn (length l1) l – n - k ↓.
+Proof.
+  induction k; intros; inversion H0; subst; auto.
+  * rewrite Nat.sub_0_r. auto.
+  * replace (n - S k) with ((n - 1) - k) by lia. destruct s.
+    - eapply terminates_step with (n := n) (l' := Some s) in H2.
+      2: exact H.
+      eapply IHk in H3. 2: exact H2. destruct l eqn:l'; simpl in *.
+      + rewrite drop_nil in H3. exact H3.
+      + exact H3.
+    - eapply terminates_step with (n := n) (l' := None) in H2.
+      2: exact H.
+      eapply IHk in H3. exact H3. exact H2.
+Qed.
+
+Corollary step_term_term :
+  forall k n fs e fs' e' l1 l2,
+  ⟨fs, e⟩ -[k , l1]->ₗ ⟨fs', e'⟩ -> | fs', e' | l2 – n - k ↓ -> n >= k 
+->
+  | fs, e | l1 ++ l2 – n ↓.
+Proof.
+  intros. apply semantic_iff_termination.
+  apply semantic_iff_termination in H0. destruct H0, H0.
+  pose proof (transitive_eval H H2). replace (k+(n-k)) with n in H3 by lia.
+  eexists. eauto.
+Qed.
+
+Corollary step_term_term_plus :
+  forall k k2 fs e fs' e' l1 l2, 
+  ⟨fs, e⟩ -[k , l1]->ₗ ⟨fs', e'⟩ -> | fs', e' | l2 – k2 ↓
+->
+  | fs, e | l1 ++ l2 – k + k2 ↓.
+Proof.
+  intros. apply semantic_iff_termination.
+  apply semantic_iff_termination in H0. destruct H0, H0.
+  pose proof (transitive_eval H H1).
+  eexists. eauto.
+Qed.
+
+Lemma create_result_is_not_box :
+  forall ident vl r eff',
+  ICLOSED ident ->
+  Forall (fun v => VALCLOSED v) vl ->
+  Some (r, eff') = create_result ident vl ->
+  is_result r \/
+  (exists e, r = RExp e).
+Proof.
+  destruct ident; intros; simpl in *; try invSome; auto.
+  1: left; do 2 constructor; auto; constructor; now apply indexed_to_forall.
+  1: left; do 2 constructor. constructor; auto.
+  (* map *)
+  1-2: erewrite <- length_map; apply indexed_to_forall.
+  1-2: eapply List.Forall_map; apply make_val_map_keeps_prop.
+  1-2: eapply Forall_impl; [|eapply deflatten_keeps_prop; eassumption].
+  1-2: intros; destruct a; apply H1.
+  (****)
+  1: auto.
+  1: left; destruct m, f; try destruct l; try destruct l0; try invSome; try constructor; inv H; scope_solver.
+  1: symmetry in H1; eapply eval_is_result in H1; auto.
+  * left. destruct (primop_eval f vl) eqn: pe.
+    - inv H1. eapply primop_eval_is_result; eassumption.
+    - inv H1.
+  * inv H. destruct v; try invSome; try now (left; constructor; auto).
+    break_match_hyp; invSome; auto.
+    right. eexists. reflexivity.
+    left. constructor; auto.
+Qed.
+
+From CoreErlang.FrameStack Require Export
+  SubstSemanticsLabeled.
+
+Lemma Private_params_exp_eval :
+  forall exps ident vl Fs (e : Exp) n (Hid : ICLOSED ident) (l : SideEffectList) (Hvl : Forall (fun v => VALCLOSED v) vl),
+  | FParams ident vl exps :: Fs, e | l – n ↓ ->
+  (forall m : nat,
+  m < S n ->
+  forall (Fs : FrameStack) (e : Exp) (ll : SideEffectList),
+  | Fs, e | ll – m ↓ ->
+  exists (res : Redex) (k : nat) (l : SideEffectList),
+    is_result res /\ ⟨ [], e ⟩ -[ k , l ]->ₗ ⟨ [], res ⟩ /\ k <= m) ->
+  exists res k l, is_result res /\
+  ⟨ FParams ident vl exps :: Fs, e⟩ -[k , l]->ₗ
+  ⟨ Fs, res ⟩ /\ k <= n.
+Proof.
+  induction exps; intros.
+  * apply H0 in H as H'. 2: lia.
+    destruct H' as [res [k [ll [Hres [Hd Hlt]]]]].
+    eapply frame_indep_nil in Hd.
+(*    specialize (H1 _ _ _ _ _ Hd).
+    eapply H1 in H. *)
+    eapply term_step_term_2 in H. 2: exact Hd. simpl in *.
+    inv Hres.
+    - do 3 eexists. split. 2: split.
+      2: {
+        eapply transitive_eval. exact Hd.
+        eapply step_trans. constructor. reflexivity. apply step_refl.
+        reflexivity.
+      }
+      auto.
+      inv H. lia.
+    - destruct vs. 2: destruct vs. 1, 3: inv H. (* vs is a singleton *)
+      inv H. destruct (create_result_is_not_box ident (vl ++ [v]) res l0); auto.
+      + now apply Forall_app.
+      + do 3 eexists. split. 2: split.
+        2: {
+          eapply transitive_eval. exact Hd.
+          eapply step_trans. econstructor. eassumption. apply step_refl.
+          reflexivity.
+        }
+        auto.
+        lia.
+      (* if create_result was a function application: *)
+      + inv H. apply H0 in H9 as H9'.
+        destruct H9' as [res2 [k2 [l2 [Hres2 [Hd2 Hlt2]]]]]. 2: lia.
+        eapply frame_indep_nil in Hd2.
+        eapply term_step_term_2 in H9. 2: exact Hd2.
+        do 3 eexists. split. 2: split.
+        2: {
+          eapply transitive_eval. exact Hd.
+          eapply step_trans. econstructor. eassumption.
+          exact Hd2. reflexivity.
+        }
+        auto.
+        lia.
+  * (* same as above *)
+    apply H0 in H as H'. 2: lia.
+    destruct H' as [res [k [ll [Hres [Hd Hlt]]]]].
+    eapply frame_indep_nil in Hd.
+    eapply term_step_term_2 in H. 2: exact Hd. simpl in *.
+    inv Hres.
+    - do 3 eexists. split. 2: split.
+      2: {
+        eapply transitive_eval. exact Hd.
+        eapply step_trans. constructor. reflexivity. apply step_refl.
+        reflexivity.
+      }
+      auto.
+      inv H. lia.
+    (* up to this point*)
+    - destruct vs. 2: destruct vs. 1, 3: inv H.
+      inv H. apply IHexps in H9 as [res2 [k2 [l2 [Hres2 [Hd2 Hlt2]]]]].
+      4: {
+        intros. eapply H0. lia. eassumption.
+      }
+      do 3 eexists. split. 2: split.
+      2: {
+        eapply transitive_eval. exact Hd.
+        eapply step_trans. constructor. exact Hd2.
+        reflexivity.
+      }
+      auto.
+      lia.
+      auto.
+      now apply Forall_app.
+Qed.
+
+Theorem prefix_drop : forall {A} (l0 l1 : list A) ,
+            l0 `prefix_of` l1 -> 
+            forall l2,
+              l2 = drop (length l0) l1 ->
+              l1 = l0 ++ l2 .
+Proof.
+  induction l0; intros; subst.
+  - simpl. rewrite drop_0. reflexivity.
+  - inv H. simpl. rewrite drop_app_length.
+    reflexivity.
+Qed.
+
+Lemma Private_params_exp_eval_empty :
+  forall exps ident vl Fs (e : Exp) n l (Hid : ICLOSED ident) (Hvl : Forall (fun v => VALCLOSED v) vl) (Hcle : EXPCLOSED e) (Hexps : Forall (fun e => EXPCLOSED e) exps),
+  | FParams ident vl exps :: Fs, e | l – n ↓ ->
+  (forall m : nat,
+  m < S n ->
+  forall (Fs : FrameStack) (e : Exp) (l : SideEffectList),
+  | Fs, e | l – m ↓ -> EXPCLOSED e ->
+  exists (res : Redex) (k : nat) (l' : SideEffectList),
+    is_result res /\ ⟨ [], e ⟩ -[ k , l' ]->ₗ ⟨ [], res ⟩ /\ k <= m /\ l' `prefix_of` l) ->
+  exists res k l', is_result res /\
+  ⟨ [FParams ident vl exps], e⟩ -[k , l']->ₗ
+  ⟨ [], res ⟩ /\ k <= n /\ l' `prefix_of` l.
+Proof.
+  induction exps; intros.
+  * apply H0 in H as H'. 2: lia. 2: assumption.
+    destruct H' as [res [k [l' [Hres [Hd [Hlt Hpref]]]]]].
+    eapply frame_indep_nil in Hd as Hlia.
+    eapply frame_indep_nil in Hd.
+    eapply term_step_term_2 in H as Hlia2. 2: exact Hlia. simpl in *.
+    inv Hres.
+    - do 3 eexists. split. 2: split. 3: split.
+      2: {
+        eapply transitive_eval. exact Hd.
+        eapply step_trans. constructor. reflexivity. apply step_refl.
+        reflexivity.
+      }
+      auto.
+      inv Hlia2. lia.
+      rewrite app_nil_r. assumption.
+    - destruct vs. 2: destruct vs. 1, 3: inv Hlia2. (* vs is a singleton *)
+      inv Hlia2. destruct (create_result_is_not_box ident (vl ++ [v]) res l0).
+      + auto.
+      + now apply Forall_app.
+      + eassumption.
+      + do 3 eexists. split. 2: split. 3: split.
+        2: {
+          eapply transitive_eval. exact Hd.
+          eapply step_trans. econstructor. eassumption. apply step_refl.
+          reflexivity.
+        }
+        auto.
+        lia.
+        unfold option_cons in *.
+        destruct l0. 2: rewrite app_nil_r; assumption.
+        rewrite (prefix_drop _ _ Hpref _ H7).
+        rewrite (cons_middle s l' ls). rewrite app_assoc.
+        apply prefix_app_r. auto.
+      (* if create_result was a function application: *)
+      + inv H2. apply H0 in H9 as H9'. 2: lia.
+        destruct H9' as [res2 [k2 [l2 [Hres2 [Hd2 [Hlt2 Hpref2]]]]]].
+        eapply frame_indep_nil in Hd2 as Hlia3.
+        eapply frame_indep_nil in Hd2.
+        eapply term_step_term_2 in H9. 2: exact Hlia3.
+        do 3 eexists. split. 2: split. 3: split.
+        2: {
+          eapply transitive_eval. exact Hd.
+          eapply step_trans. econstructor. eassumption.
+          exact Hd2. reflexivity.
+        }
+        auto.
+        lia. subst.
+        2: { 
+          pose proof (create_result_closed
+                            (vl ++ [v])
+                            ident
+                            x
+                            l0
+                            ltac:(apply Forall_app; auto)
+                            Hid
+                            H4).
+          by inversion H2.
+        }
+        unfold option_cons in *.
+        destruct l0; rewrite (prefix_drop _ _ Hpref _ H7).
+        ** do 2 rewrite cons_middle.
+           apply prefix_app.
+           apply prefix_app.
+           assumption.
+        ** apply prefix_app.
+           assumption.
+  * (* same as above *)
+    apply H0 in H as H'. 2: lia.
+    destruct H' as [res [k [l' [Hres [Hd Hlt]]]]].
+    eapply frame_indep_nil in Hd as Hlia.
+    eapply frame_indep_nil in Hd.
+    eapply term_step_term_2 in H as Hlia2. 2: exact Hlia. simpl in *.
+    inv Hres.
+    - do 3 eexists. split. 2: split. 3: split.
+      2: {
+        eapply transitive_eval. exact Hd.
+        eapply step_trans. constructor. reflexivity. apply step_refl.
+        reflexivity.
+      }
+      auto.
+      inv Hlia2. lia.
+      destruct Hlt.
+      rewrite app_nil_r.
+      assumption.
+    (* up to this point*)
+    - destruct vs. 2: destruct vs. 1, 3: inv Hlia2.
+      inv Hlia2. inv H1. inv Hexps.
+      apply IHexps in H9 as [res2 [k2 [l2 [Hres2 [Hd2 Hlt2]]]]]; auto.
+      3: {
+        intros. eapply H0. lia. eassumption. eassumption.
+      }
+      do 3 eexists. split. 2: split. 3: split.
+      2: {
+        eapply transitive_eval. exact Hd.
+        eapply step_trans. constructor.
+        exact Hd2.
+        reflexivity.
+      }
+      auto.
+      lia.
+      auto.
+      destruct Hlt2. destruct Hlt.
+      inv H8. apply prefix_app.
+      rewrite drop_app_length in H2.
+      assumption.
+      apply Forall_app. split; auto.
+    - auto.
+Qed.
+
+(**
+  so far
+*)
+
+Lemma term_empty : forall x Fs (e : Exp) (He : EXPCLOSED e) (l : SideEffectList),
+  | Fs, e | l – x ↓ ->
+  exists k l', | [], e | l' – k ↓ /\ k <= x /\ l' `prefix_of` l.
+Proof.
+  induction x using Wf_nat.lt_wf_ind; intros; inv H0.
+  * do 2 eexists. split. constructor; auto. constructor. auto. split.
+    lia. apply prefix_nil.
+  * destruct el. (* tricks to avoid RBox *)
+    - do 2 eexists. split. constructor.
+      epose proof (cool_params_0_l [] IValues [] _ None []). simpl in H0.
+      eapply H0.
+      congruence. reflexivity. do 2 constructor. auto. inv H3. split. lia.
+      apply prefix_nil.
+    - inv H3. destruct_scopes.
+      eapply Private_params_exp_eval_empty in H9 as HH2; auto.
+      2-3: rewrite <- indexed_to_forall in H3; now inv H3.
+      2: {
+        intros. epose proof (H m ltac:(slia) Fs0 e0 _ _ H1) as [j [l' [HD [Hj Hpref]]]].
+        apply semantic_iff_termination in HD as [res [Hres Hr]].
+        do 3 eexists. split. 2: split. 3: split. all: eassumption.
+      }
+      destruct HH2 as [res [k [l' [Hres [Hd [Hlt Hpref]]]]]].
+      do 2 eexists. split. do 2 constructor. congruence.
+      eapply semantic_iff_termination. eexists.
+      split. 2: exact Hd. auto. split. lia. assumption.
+  * destruct el. (* proof is same as above, tricks to avoid RBox *)
+    - do 2 eexists. split. constructor.
+      epose proof (cool_params_0_l [] ITuple [] _ None []). simpl in H0.
+      eapply H0.
+      congruence. reflexivity. do 4 constructor; auto. intros. inv H1. inv H3.
+      split. lia. apply prefix_nil.
+    - inv H3. destruct_scopes.
+      eapply Private_params_exp_eval_empty in H9 as HH2; auto.
+      2-3: rewrite <- indexed_to_forall in H3; now inv H3.
+      2: {
+        intros. epose proof (H m ltac:(slia) Fs0 e0 _ _ H1) as [j [l' [HD [Hj Hpref]]]].
+        apply semantic_iff_termination in HD as [res [Hres Hr]].
+        do 3 eexists. split. 2: split. 3: split. all: eassumption.
+      }
+      destruct HH2 as [res [k [l' [Hres [Hd [Hlt Hpref]]]]]].
+      do 2 eexists. split. do 2 constructor. congruence.
+      eapply semantic_iff_termination. eexists.
+      split. 2: exact Hd. auto. split. lia. assumption.
+  * do 2 eexists. split. do 5 constructor; slia. split. lia. apply prefix_nil.
+  * destruct_scopes.
+    eapply Private_params_exp_eval_empty in H3 as HH2; auto.
+    2: apply (H1 0); slia.
+    2: { constructor. apply (H5 0); slia. apply flatten_keeps_prop.
+         rewrite indexed_to_forall with (def := (˝VNil, ˝VNil)). intros.
+         specialize (H1 (S i) ltac:(slia)). specialize (H5 (S i) ltac:(slia)).
+         simpl in *. rewrite map_nth with (d := (˝VNil, ˝VNil)) in H1, H5.
+         destruct nth; now split.
+       }
+    2: {
+      intros. epose proof (H m ltac:(slia) Fs0 e _ _ H2) as [j [l' [HD [Hj Hpref]]]].
+      apply semantic_iff_termination in HD as [res [Hres Hr]].
+      do 3 eexists. split. 2: split. 3: split. all: eassumption.
+    }
+    destruct HH2 as [res [k0 [l' [Hres [Hd [Hlt Hpref]]]]]].
+    do 2 eexists. split. constructor.
+    eapply semantic_iff_termination. eexists.
+    split. 2: exact Hd. auto. split. lia. assumption.
+  * (* Call is trickier, because first the module, then the function
+       expression has to be evaluated *)
+    destruct_scopes. apply H in H3 as HD1; auto.
+    destruct HD1 as [k1 [l1 [D1 [Hlia1 Hpref]]]].
+    apply semantic_iff_termination in D1 as [res1 [Hres1 Hr1]].
+    eapply frame_indep_nil in Hr1 as Hr1'.
+    eapply frame_indep_nil in Hr1.
+    eapply term_step_term_2 in H3.
+    2: exact Hr1. simpl in *.
+    inv Hres1.
+    (* moduleexp Exception *)
+    - inv H3. do 2 eexists. split. constructor.
+      eapply step_term_term_plus. exact Hr1'. constructor.
+      congruence. constructor. constructor; auto. split. lia.
+      rewrite app_nil_r. assumption.
+    (* moduleexp Value *)
+    - inv H3. inv H0. (* clear H5. *)
+      apply H in H10 as HD2; auto. 2: lia.
+      destruct HD2 as [k2 [l2 [D2 [Hlia2 Hpref2]]]].
+      apply semantic_iff_termination in D2 as [res2 [Hres2 Hr2]].
+      eapply frame_indep_nil in Hr2 as Hr2'.
+      eapply frame_indep_nil in Hr2.
+      eapply term_step_term_2 in H10.
+      2: exact Hr2. simpl in *.
+      inv Hres2.
+      (* funexp exception *)
+      + inv H10. do 2 eexists. split. constructor.
+        eapply step_term_term_plus. exact Hr1'. constructor.
+        eapply step_term_term_plus. exact Hr2'. constructor.
+        congruence. constructor. constructor; auto. split. lia.
+        rewrite app_nil_r. destruct Hpref2. symmetry in H2.
+        epose proof (prefix_drop l1 l Hpref (l2 ++ x) H2).
+        rewrite H5. Search (_ ++ _ `prefix_of` _ ++ _).
+        apply prefix_app. rewrite <- app_nil_r at 1. apply prefix_app.
+        apply prefix_nil.
+      (* moduleexp value *)
+      + inv H10. destruct el. (* tricks to avoid RBox *)
+        ** inv H13. do 2 eexists. split.
+           constructor.
+           eapply step_term_term_plus. exact Hr1'. constructor.
+           eapply step_term_term_plus. exact Hr2'. constructor.
+           epose proof (cool_params_0_l [] (ICall v f0) [] _ l0 []). simpl in H1.
+           apply H1.
+           congruence. exact H12. clear H1.
+           (* here is this different from the previous *)
+           simpl in H12. destruct_foralls.
+           destruct v, f0; try destruct l; try destruct l0; try destruct l3; try invSome; try constructor; auto.
+           all: try (constructor; constructor; apply indexed_to_forall);
+             try (constructor; [|constructor]; auto).
+           -- destruct l4.
+              ++ eapply (eval_is_result ); eauto.
+              ++ inv H12.
+           -- destruct l4 eqn: a.
+              ++ eapply (eval_is_result ); eauto.
+              ++ inv H12. unfold badfun.
+                 eapply exception_is_result. auto. scope_solver.
+           -- destruct l4.
+              ++ eapply (eval_is_result ); eauto.
+              ++ inv H12.
+           -- destruct l4.
+              ++ eapply (eval_is_result ); eauto.
+              ++ inv H12.
+                 eapply exception_is_result. auto. scope_solver.
+           -- split. lia. destruct l0; simpl in H9; simpl.
+              ++ destruct Hpref2. rewrite H1 in H9.
+                 symmetry in H1.
+                 epose proof (prefix_drop _ _ Hpref _ H1). rewrite H2.
+                 apply prefix_app. apply prefix_app. rewrite drop_app_length in H9.
+                 rewrite <- H9.
+                 assert (s :: ls = [s] ++ ls). {
+                   simpl. reflexivity.
+                 } rewrite H5.
+                 rewrite <- app_nil_r at 1. apply prefix_app. apply prefix_nil.
+              ++ destruct Hpref2. rewrite H1 in H9.
+                 symmetry in H1.
+                 epose proof (prefix_drop _ _ Hpref _ H1). rewrite H2.
+                 apply prefix_app. apply prefix_app. apply prefix_nil.
+        ** inv H13. inv H0.
+           eapply Private_params_exp_eval_empty in H17 as HD3; auto.
+           2: {
+             apply (H6 0). slia.
+           }
+           2: {
+             apply indexed_to_forall in H6. now inv H6.
+           }
+           2: {
+             intros. epose proof (H m0 ltac:(slia) Fs0 e0 _ _ H1) as [j [ls [HD [Hj Hpref3]]]].
+             apply semantic_iff_termination in HD as [res [Hres Hr]].
+             do 3 eexists. split. 2: split. 3: split. all: eassumption.
+           }
+           destruct HD3 as [res3 [k3 [l3 [Hres3 [Hd3 [Hlt3 Hpref3]]]]]].
+           do 2 eexists. split. 2: split.
+           constructor.
+           eapply step_term_term_plus. exact Hr1'. constructor.
+           eapply step_term_term_plus. exact Hr2'. constructor.
+           constructor. congruence.
+           eapply semantic_iff_termination. eexists.
+           split. 2: exact Hd3. auto. lia.
+           destruct Hpref. subst.
+           apply prefix_app. rewrite drop_app_length in *.
+           destruct Hpref2. subst.
+           apply prefix_app. rewrite drop_app_length in *.
+           destruct Hpref3. subst.
+           rewrite app_nil_end_deprecated at 1.
+           apply prefix_app. apply prefix_nil.
+  * destruct el. (* tricks to avoid RBox *)
+    - inv H3. do 2 eexists. split. constructor. eapply cool_params_0_l.
+      congruence. eassumption.
+      (* here is this different from the previous *)
+      simpl. constructor. 2: split. 2: lia. cbn in H5.
+      destruct (primop_eval f []) eqn: pe. 2: invSome.
+      destruct p. inv H5. eapply primop_eval_is_result with (f:=f); eauto.
+      destruct l0; simpl.
+      + assert (s :: ls = [s] ++ ls). {
+                simpl. reflexivity.
+               }
+        rewrite H0.
+        rewrite app_nil_end_deprecated at 1.
+        apply prefix_app. apply prefix_nil.
+      + apply prefix_nil.
+    - inv H3. destruct_scopes.
+      eapply Private_params_exp_eval_empty in H9 as HH2; auto.
+      2-3: rewrite <- indexed_to_forall in H3; now inv H3.
+      2: {
+        intros. epose proof (H m ltac:(slia) Fs0 e0 _ _ H1) as [j [l1 [HD [Hj Hpref]]]].
+        apply semantic_iff_termination in HD as [res [Hres Hr]].
+        do 3 eexists. split. 2: split. 3: split. all: eassumption.
+      }
+      destruct HH2 as [res [k [l1 [Hres [Hd [Hlt Hpref]]]]]].
+      do 2 eexists. split. do 2 constructor. congruence.
+      eapply semantic_iff_termination. eexists.
+      split. 2: exact Hd. auto. split. lia. assumption.
+  (* application is harder, because first, the function parameter needs
+     to be evaluated, then we do a case separation, whether l = [].
+     Everytime an exception occurs, that needs to be propagated -> hence
+     the number of case separations. *)
+  * apply H in H3 as H3'. destruct H3' as [j [l1 [Hj [Hlt1 Hpref]]]]. 2: lia.
+    apply semantic_iff_termination in Hj as [res [Hres Hr]].
+    eapply frame_indep_nil in Hr as Hlia1.
+    eapply frame_indep_nil in Hr. eapply term_step_term_2 in H3.
+    2: exact Hlia1. simpl in *.
+    destruct l. (* tricks to avoid RBox *)
+    - inv Hres. (* exception result? *)
+      + exists (2 + j). eexists. split. constructor.
+        eapply step_term_term. simpl. exact Hr. 2: lia.
+        replace (S j - j) with 1 by lia.
+        constructor. reflexivity. constructor. auto.
+        inv H3. split. lia.
+        rewrite app_nil_r. assumption.
+      + do 2 eexists.
+        split. 2: split. 3: exact Hpref. constructor. inv H3. inv H6.
+        
+        
+        all: admit.
+        (**
+         destruct (create_result_is_not_box (IApp v) [] res l1).
+        ** inv H0; now constructor.
+        ** auto.
+        ** assumption.
+        ** exists (3 + j). split. constructor.
+           eapply step_term_term. exact Hr. 2: lia.
+           replace (S (S j) - j) with 2 by lia.
+           constructor. econstructor. congruence. eassumption.
+           now constructor.
+           lia.
+        ** inv H1. apply H in H9 as H9'. 2: lia.
+           destruct H9' as [i [Hd2 Hlt2]].
+           exists (1 + (j + 2 + i)). split. constructor.
+           eapply step_term_term. exact Hr. 2: lia.
+           replace (j + 2 + i - j) with (2 + i) by lia.
+           constructor. econstructor. congruence. eassumption.
+           assumption. lia.
+           inv H0.
+           pose proof (create_result_closed [] (IApp v) x l ltac:(auto) ltac:(now constructor) H7). now inv H0. *)
+    - inv Hres.
+      + exists (2 + j). eexists. split. constructor.
+        eapply step_term_term. exact Hr. 2: lia.
+        replace (S j - j) with 1 by lia.
+        constructor. reflexivity. constructor. auto.
+        inv H3. split. lia. rewrite app_nil_r. assumption.
+      + inv H3. admit.
+      
+        (**
+        inv H2. destruct_scopes.
+        eapply Private_params_exp_eval_empty in H10 as HH2; auto.
+        3-4: rewrite <- indexed_to_forall in H7; now inv H7.
+        2: { inv H0; now constructor. }
+        2: {
+          intros. epose proof (H m ltac:(slia) Fs0 e1 _ H2) as [i [Hd2 Hi]].
+          apply semantic_iff_termination in Hd2
+             as [res2 [Hres2 Hr2]].
+          do 2 eexists. split. 2: split. all: eassumption.
+        }
+        destruct HH2 as [res2 [i [Hres2 [Hd2 Hlt2]]]].
+        assert (⟨ [FApp1 (e :: l)], RValSeq [v]⟩ -[2]-> ⟨ [FParams (IApp v) [] l], e ⟩). {
+          repeat econstructor. congruence.
+        }
+        eapply (transitive_eval Hr) in H1.
+        eapply (transitive_eval H1) in Hd2.
+        eexists. split.
+        constructor. apply semantic_iff_termination.
+        eexists. split. 2: exact Hd2. assumption. lia.
+        *)
+    - now destruct_scopes.
+  * apply H in H3 as HH. 2: lia.
+    destruct HH as [i [li [Hi [Hlt Hprefi]]]].
+    apply semantic_iff_termination in Hi as [res [Hres Hr]].
+    eapply frame_indep_nil in Hr as Hlia1.
+    eapply frame_indep_nil in Hr.
+    eapply term_step_term_2 in H3. 2: exact Hlia1.
+    inv Hres. (* tail exception or not *)
+    - exists (S i + 1). eexists.
+      split. 2: split. 2: inv H3; lia.
+      simpl. constructor. apply semantic_iff_termination.
+      exists (RExc (cl, v1, v2)). split; auto. eapply transitive_eval.
+      exact Hr. do 2 econstructor. reflexivity.
+      rewrite app_nil_r. assumption.
+    - inv H3. apply H in H6 as HH. 2: lia.
+      destruct HH as [j [lj [Hj [Hltj Hprefj]]]].
+      simpl in *. apply semantic_iff_termination in Hj as [hdres [Hr2 Hd2]].
+      eapply frame_indep_nil in Hd2 as Hlia2.
+      eapply frame_indep_nil in Hd2.
+      eapply term_step_term_2 in H6. 2: exact Hlia2.
+      assert (⟨ [FCons1 hd], RValSeq [tl0] ⟩ -[1 , []]->ₗ ⟨[FCons2 tl0], hd⟩). {
+        repeat econstructor.
+      }
+      eapply (transitive_eval Hr) in H1.
+      eapply (transitive_eval H1) in Hd2.
+      inv Hr2. (* head exception or not *)
+      + exists (1 + (i + (1 + (j + 1) ))). eexists. split.
+        simpl. constructor. eapply step_term_term.
+        exact Hd2.
+        replace (i + S (j + 1) - (i + 1 + j)) with 1 by lia.
+        constructor. reflexivity. do 2 constructor; auto.
+        lia. split.
+        inv H6. simpl. lia.
+        repeat (rewrite app_nil_r).
+        destruct Hprefi. rewrite H4 in *. apply prefix_app.
+        destruct Hprefj. rewrite drop_app_length in H5. rewrite H5.
+        rewrite <- app_nil_r at 1. apply prefix_app. apply prefix_nil.
+      + exists (1 + (i + (1 + (j + 1) ))). eexists. split.
+        simpl. constructor. eapply step_term_term.
+        exact Hd2. inv H1.
+        replace (i + S (j + 1) - (i + 1 + j)) with 1 by lia.
+        
+        
+        
+        all: admit.
+        (**
+        constructor. do 4 constructor; inv H0; now inv H3.
+        lia.
+        inv H2. lia.
+        *)
+      + now destruct_scopes.
+    - now destruct_scopes.
+  * apply H in H3 as HH. 2: lia.
+    destruct HH as [i [li [Hi [Hlt Hprefi]]]].
+    apply semantic_iff_termination in Hi as [res [Hres Hr]].
+    eapply frame_indep_nil in Hr as Hlia1.
+    eapply frame_indep_nil in Hr.
+    eapply term_step_term_2 in H3. 2: exact Hlia1.
+    inv Hres. (* tail exception or not *)
+    - exists (S i + 1). eexists.
+      split. 2: split. 2: inv H3; lia.
+      simpl. constructor. apply semantic_iff_termination.
+      exists (RExc (cl, v1, v2)). split; auto. eapply transitive_eval.
+      exact Hr. do 2 econstructor. reflexivity.
+      rewrite app_nil_r. assumption.
+    - inv H3. apply H in H9 as HH. 2: lia.
+      destruct HH as [j [lj [Hj [Hltj Hprefj]]]].
+      simpl in *. apply semantic_iff_termination in Hj as [hdres [Hr2 Hd2]].
+      eapply frame_indep_nil in Hd2 as Hlia2.
+      eapply term_step_term_2 in H9. 2: exact Hlia2.
+      assert (⟨ [FLet (Datatypes.length vs) e2], RValSeq vs ⟩ -[1, []]->ₗ 
+      ⟨ [], e2.[list_subst vs idsubst] ⟩). {
+        repeat econstructor.
+      }
+      eapply (transitive_eval Hr) in H1.
+      eapply (transitive_eval H1) in Hd2.
+      exists (1 + (i + (1 + j))). eexists. split. 2: split. 2: inv Hr2; inv H1; lia.
+      constructor. eapply step_term_term. exact Hd2.
+      replace (i + (1 + j) - (i + 1 + j)) with 0 by lia.
+      now constructor.
+      lia.
+      repeat (rewrite app_nil_r).
+      destruct Hprefi. rewrite H2 in *. apply prefix_app.
+      destruct Hprefj. rewrite drop_app_length in H3. rewrite H3.
+      rewrite <- app_nil_r at 1. apply prefix_app. apply prefix_nil.
+      destruct_scopes. apply -> subst_preserves_scope_exp; eauto.
+      rewrite Nat.add_0_r. now apply scoped_list_idsubst.
+    - now destruct_scopes.
+  (* Sequencing is basically same as let *)
+  * apply H in H3 as HH. 2: lia.
+    destruct HH as [i [li [Hi [Hlt Hprefi]]]].
+    apply semantic_iff_termination in Hi as [res [Hres Hr]].
+    eapply frame_indep_nil in Hr as Hlia1.
+    eapply frame_indep_nil in Hr.
+    eapply term_step_term_2 in H3. 2: exact Hlia1.
+    inv Hres. (* tail exception or not *)
+    - exists (S i + 1). eexists.
+      split. 2: split. 2: inv H3; lia.
+      simpl. constructor. apply semantic_iff_termination.
+      exists (RExc (cl, v1, v2)). split; auto. eapply transitive_eval.
+      exact Hr. do 2 econstructor. reflexivity.
+      rewrite app_nil_r. assumption.
+    - inv H3. apply H in H6 as HH. 2: lia.
+      destruct HH as [j [lj [Hj [Hltj Hprefj]]]].
+      simpl in *. apply semantic_iff_termination in Hj as [hdres [Hr2 Hd2]].
+      eapply frame_indep_nil in Hd2 as Hlia2.
+      eapply term_step_term_2 in H6. 2: exact Hlia2.
+      assert (⟨ [FSeq e2], RValSeq [v] ⟩ -[1 , []]->ₗ
+      ⟨ [], e2 ⟩). {
+        repeat econstructor.
+      }
+      eapply (transitive_eval Hr) in H1.
+      eapply (transitive_eval H1) in Hd2.
+      exists (1 + (i + (1 + j))). eexists. split. 2: split. 2: inv Hr2; inv H1; lia.
+      constructor. eapply step_term_term. exact Hd2.
+      replace (i + (1 + j) - (i + 1 + j)) with 0 by lia.
+      now constructor.
+      lia.
+      repeat (rewrite app_nil_r).
+      destruct Hprefi. rewrite H2 in *. apply prefix_app.
+      destruct Hprefj. rewrite drop_app_length in H3. rewrite H3.
+      rewrite <- app_nil_r at 1. apply prefix_app. apply prefix_nil.
+      now destruct_scopes.
+    - now destruct_scopes.
+  * do 2 eexists. split. constructor. do 3 constructor; auto.
+    destruct_scopes. constructor; intros. inv H0. auto. split. lia.
+    apply prefix_nil.
+  (* for case: list_length_ind on H3 (or structural could also be enough) *)
+  * apply H in H3 as HH. 2: lia. destruct HH as [k1 [l1 [Hd1 [Hlt1 Hpref1]]]].
+    apply semantic_iff_termination in Hd1 as [r1 [Hr Hd]].
+    eapply frame_indep_nil in Hd as Hlia1.
+    eapply frame_indep_nil in Hd.
+    eapply term_step_term_2 in H3. 2: exact Hlia1.
+    simpl in *.
+    inv Hr. (* exception? *)
+    + exists (1 + k1 + 1). eexists. split. 2: split. 2: inv H3; lia.
+      simpl. constructor. eapply step_term_term. exact Hd.
+      replace (k1 + 1 - k1) with 1 by lia.
+      constructor. reflexivity. do 2 constructor; auto. lia.
+      rewrite app_nil_r. assumption.
+      (**
+        so far
+      *)
+    + epose proof (Private_term_empty_case l Fs vs (k - k1) _ _ _ H3) as
+        [res [k2 [Hres [Hd2 Hlt2]]]].
+      Unshelve. 10: {
+        intros. eapply H. lia. 2: eassumption. auto.
+      }
+      pose proof (transitive_eval Hd Hd2).
+      exists (S (k1 + k2)). split. 2: lia.
+      constructor.
+      apply semantic_iff_termination. exists res. now split.
+      all: auto.
+      destruct_scopes. rewrite indexed_to_forall with (def := ([], ˝VNil, ˝VNil)).
+      intros. apply H7 in H1 as H1'. apply H8 in H1. clear H7 H8.
+      rewrite map_nth with (d := ([], ˝VNil, ˝VNil)) in H1, H1'.
+      extract_map_fun F. replace (˝VNil) with (F ([], ˝VNil, ˝VNil)) in H1' at 3 by now subst F. subst F. rewrite map_nth in H1'.
+      extract_map_fun F. replace [] with (F ([], ˝VNil, ˝VNil)) in H1 by now subst F. subst F. rewrite map_nth in H1.
+      destruct nth, p; split; cbn in *; rewrite Nat.add_0_r in *. apply H1'. apply H1.
+    + now destruct_scopes.
+  * apply H in H4 as [i [Hd Hlt]].
+    eexists. split. econstructor. reflexivity. exact Hd. lia. lia.
+    apply -> subst_preserves_scope_exp. destruct_scopes. apply H6.
+    apply scoped_list_subscoped_eq. unfold convert_to_closlist. now do 2 rewrite length_map. 2: auto.
+    apply closlist_scope. rewrite length_map, map_map; intros. destruct_scopes.
+    apply H6 in H0. clear -H0. rewrite map_map.
+    do 2 rewrite map_nth with (d := (0, ˝VNil)) in H0.
+    do 2 rewrite map_nth with (d := (0, ˝VNil)). destruct nth. now cbn in *.
+  * apply H in H3 as HH. 2: lia.
+    destruct HH as [i [Hd Hlt]].
+    apply semantic_iff_termination in Hd as [r [Hres Hd]].
+    eapply frame_indep_nil in Hd as Hlia.
+    eapply frame_indep_nil in Hd.
+    eapply term_step_term in H3. 2: exact Hlia.
+    simpl in *.
+    inv Hres. (* exception or not *)
+    - inv H3. (* 2: { inv H7. } *)
+      apply H in H4 as [j [Hd2 Hlt2]]. 2: lia.
+      exists (1 + (i + (1 + j))). split. 2: lia.
+      constructor. eapply step_term_term. exact Hd. 2: lia.
+      replace (i + (1 + j) - i) with (S j) by lia.
+      now constructor.
+      destruct_scopes. apply -> subst_preserves_scope_exp; eauto.
+      apply cons_scope. destruct cl; simpl; auto.
+      apply cons_scope. auto.
+      apply cons_scope. auto.
+      auto.
+    - inv H3.
+      apply H in H10 as [j [Hd2 Hlt2]]. 2: lia.
+      exists (1 + (i + (1 + j))). split. 2: lia.
+      constructor. eapply step_term_term. exact Hd. 2: lia.
+      replace (i + (1 + j) - i) with (S j) by lia.
+      now constructor.
+      destruct_scopes. apply -> subst_preserves_scope_exp. eauto.
+      rewrite Nat.add_0_r. now apply scoped_list_idsubst.
+    - now destruct_scopes.
+  * eexists. split. now constructor. lia.
+Unshelve.
+  all: auto.
+Qed.
+
+(* NOTE: This is not a duplicate! Do not remove! *)
+(* sufficient to prove it for Exp, since value sequences and
+   exceptions terminate in 0/1 step by definition in the
+   empty stack (and RBox does not terminate!). *)
+Corollary term_eval_empty : forall x Fs (e : Exp) (He : EXPCLOSED e),
+  | Fs, e | x ↓ ->
+  exists res k, is_result res /\ ⟨ [], e ⟩ -[k]-> ⟨ [], res ⟩ /\ k <= x.
+Proof.
+  intros. apply term_empty in H; auto. destruct H as [k [H Hlt]].
+  apply semantic_iff_termination in H as [r [Hr H]].
+  do 2 eexists; eauto.
+Qed.
+
+Corollary term_eval : forall x Fs (e : Exp) (He : EXPCLOSED e), | Fs, e | x ↓ ->
+  exists v k, is_result v /\ ⟨ Fs, e ⟩ -[k]-> ⟨ Fs, v ⟩ /\ k <= x.
+Proof.
+  intros.
+  apply term_eval_empty in H as [r [k [Hr [Hd Hlt]]]].
+  exists r, k. intuition.
+  eapply frame_indep_nil in Hd. exact Hd. auto.
+Qed.
+
+Corollary term_eval_both : forall x Fs (e : Exp) (He : EXPCLOSED e), | Fs, e | x ↓ ->
+  exists v k, is_result v /\
+  ⟨ [], e ⟩ -[k]-> ⟨ [], v ⟩ /\
+  ⟨ Fs, e ⟩ -[k]-> ⟨ Fs, v ⟩ /\ k <= x.
+Proof.
+  intros. apply term_eval_empty in H as [r [k [Hr [Hd Hlt]]]].
+  exists r, k. intuition.
+  eapply frame_indep_nil in Hd. exact Hd.
+  assumption.
+Qed.
+
+Theorem put_back : forall F e Fs (P : EXPCLOSED e) (P2 : FCLOSED F),
+  | F :: Fs, e | ↓ -> | Fs, plug_f F e | ↓.
+Proof.
+  destruct F; intros; simpl.
+  all: try now (inv H; exists (S x); constructor; auto).
+  * inv H. exists (3 + x). do 2 constructor. now inv P2.
+    now constructor.
+  * inv H. destruct ident; simpl; destruct_scopes.
+  (* These build on the same idea, however, calls, applications and maps are a bit different: *)
+  1-2, 5: destruct vl; destruct_foralls; simpl; [
+    eexists; do 2 constructor; [congruence | eassumption]
+    |
+    exists (4 + ((2 * length vl) + x)); do 2 constructor;
+    try congruence; constructor; auto;
+    eapply step_term_term;
+    [
+      apply params_eval
+      |
+      simpl app;
+      now replace (S (2 * Datatypes.length vl + x) - (1 + 2 * Datatypes.length vl)) with x by lia
+      |
+      lia
+    ]
+  ]; auto.
+    - destruct_scopes. specialize (H6 eq_refl).
+      inv H6. destruct vl.
+      + simpl. destruct el.
+        ** simpl in H. congruence.
+        ** eexists. constructor.
+           erewrite deflatten_flatten. eassumption.
+           simpl in H. instantiate (1 := x0). lia.
+      + simpl. destruct vl; simpl.
+        ** eexists. do 2 constructor. now inv H4. constructor. simpl.
+           erewrite deflatten_flatten. eassumption.
+           simpl in H. instantiate (1 := x0). lia.
+        ** exists (5 + ((2 * length vl) + x)). do 2 constructor.
+           now inv H4. do 2 constructor. now destruct_foralls.
+           erewrite deflatten_flatten.
+           2: { rewrite length_app, length_map. simpl in *.
+                instantiate (1 := x0). lia. }
+           eapply step_term_term.
+           apply params_eval. now destruct_foralls. simpl app. 2: lia.
+           now replace (S (2 * Datatypes.length vl + x) - (1 + 2 * Datatypes.length vl)) with x by lia.
+    - destruct vl; simpl.
+      + eexists. do 2 constructor. now inv H3. do 2 constructor. now inv H3.
+        do 2 constructor. congruence. eassumption.
+      + exists (8 + ((2 * length vl) + x)). do 2 constructor.
+        now inv H3. do 2 constructor. now inv H3.
+        do 2 constructor. congruence.
+        constructor. now inv H4.
+        eapply step_term_term.
+        apply params_eval. now inv H4. simpl app. 2: lia.
+        now replace (S (2 * Datatypes.length vl + x) - (1 + 2 * Datatypes.length vl)) with x by lia.
+    - destruct vl; simpl.
+      + eexists. do 2 constructor. now inv H3. do 2 constructor. congruence. eassumption.
+      + exists (6 + ((2 * length vl) + x)). do 2 constructor.
+        now inv H3. do 2 constructor. congruence.
+        constructor. now inv H4.
+        eapply step_term_term.
+        apply params_eval. now inv H4. simpl app. 2: lia.
+        now replace (S (2 * Datatypes.length vl + x) - (1 + 2 * Datatypes.length vl)) with x by lia.
+  * destruct H as [k D]. eexists. do 2 constructor. now inv P2. constructor.
+    eassumption.
+  * inv H. apply term_eval_both in H0 as H'. destruct H' as [res [l [Hres [D0 [D1 Hlt]]]]]. 2: assumption.
+    eapply term_step_term in H0. 2: eassumption.
+    clear D1. inv Hres.
+    - inv H0.
+      eexists. do 3 econstructor. congruence. reflexivity.
+      econstructor. reflexivity. cbn. eapply frame_indep_nil in D0.
+      do 2 rewrite idsubst_is_id_exp.
+      eapply step_term_term_plus. eassumption. constructor. reflexivity.
+      eassumption.
+    - inv H0.
+      + eexists. do 3 econstructor. congruence. reflexivity.
+        econstructor. reflexivity. do 2 rewrite idsubst_is_id_exp.
+        eapply frame_indep_nil in D0. eapply step_term_term_plus.
+        eassumption. econstructor. eassumption.
+      + eexists (4 + (l + (7 + 2 * length lv + k))). simpl. do 3 econstructor. congruence. reflexivity.
+        econstructor. reflexivity. do 2 rewrite idsubst_is_id_exp.
+        eapply frame_indep_nil in D0. eapply step_term_term_plus.
+        eassumption. constructor. econstructor.
+        reflexivity. cbn. do 2 constructor.
+        replace (map
+       (fun '(p, x0, y) =>
+        (p, x0.[upn (PatListScope p) idsubst],
+         y.[upn (PatListScope p) idsubst])) le) with le.
+        replace (map (fun x0 : Exp => x0.[idsubst]) (map VVal lv)) with (map VVal lv).
+        2: {
+          clear. induction lv; auto. simpl. rewrite idsubst_is_id_val.
+          now rewrite IHlv at 1.
+        }
+        2: {
+          clear. induction le; auto. simpl. destruct a, p.
+          rewrite idsubst_upn, <-IHle.
+          now do 2 rewrite idsubst_is_id_exp.
+        }
+        clear D0. do 2 econstructor.
+        destruct lv.
+        ** econstructor. congruence. reflexivity. simpl. eassumption.
+        ** simpl. constructor. congruence.
+           econstructor. inv P2. now inv H4.
+           change clock to (1 + 2 * length lv + k).
+           eapply step_term_term_plus.
+           eapply params_eval_create. inv P2. now inv H4. reflexivity.
+           cbn. eassumption.
+(*   * deriv. apply term_eval in H0 as H0'.
+    repeat destruct_hyps. eapply term_step_term in H0. 2: eassumption. 2: assumption.
+    inv H.
+    - inv H0. inv H8.
+    - inv H0.
+  * deriv. apply term_eval in H0 as H0'.
+    repeat destruct_hyps. eapply term_step_term in H0. 2: eassumption. 2: assumption.
+    inv H.
+    - inv H0. inv H8.
+    - inv H0. *)
+Qed.
+
+Theorem put_back_rev : forall F e Fs (P : EXPCLOSED e), FCLOSED F ->
+  | Fs, plug_f F e | ↓ -> | F :: Fs, e | ↓.
+Proof.
+  destruct F; intros; simpl.
+  all: try now (inv H0; cbn in *; inv_term; [eexists;eassumption | inv H0]).
+  * inv H0. cbn in *. inv H1. inv H5. inv H3. eexists. eassumption. inv H0.
+  * cbn. inv H0. destruct ident; simpl in H1.
+    1-2, 5:
+      inv_term; [
+        destruct vl; inv_term;
+         [eexists; eassumption
+         |inv H8; eapply term_step_term in H3;[|apply params_eval]]; inv H; destruct_foralls; auto;
+         eexists; eassumption
+        |inv H0
+      ].
+    (* again, map, call and apply need special care: *)
+    - destruct_scopes. specialize (H7 eq_refl). inv H7. destruct vl.
+      + destruct el.
+        ** simpl in H. congruence.
+        ** inv H1. 2: inv H0. erewrite deflatten_flatten in H9.
+           2: { instantiate (1 := x0). simpl in H. lia. }
+           eexists. eassumption.
+      + destruct vl; simpl in *.
+        ** inv H1. 2: inv H0. erewrite deflatten_flatten in H9.
+           2: { instantiate (1 := x0). simpl in H. lia. }
+           do 2 inv_term. eexists. eassumption.
+        ** inv_term. 2: inv H0. erewrite deflatten_flatten in H9.
+           2: { instantiate (1 := x0). simpl in H.
+             rewrite length_app, length_map. slia. }
+           do 3 inv_term.
+           eapply term_step_term in H7;[|apply params_eval].
+           eexists; eassumption.
+           now destruct_foralls.
+    - inv_term. 2: inv H0. do 3 inv_term. destruct vl; inv_term.
+      + inv_term. eexists. eassumption.
+      + do 2 inv_term. eapply term_step_term in H5;[|apply params_eval].
+        eexists. eassumption.
+        inv H. now destruct_foralls.
+    - inv_term. 2: inv H0. inv_term. destruct vl; inv_term.
+      + inv_term. eexists. eassumption.
+      + do 2 inv_term. eapply term_step_term in H4;[|apply params_eval].
+        eexists. eassumption.
+        inv H. now destruct_foralls.
+  * simpl in *. inv H. destruct H0 as [k D]. inv_term. 2: { inv H. }
+    do 2 inv_term. eexists. eassumption.
+  * inv H0. cbn in *. inv H1. 2: inv H0. inv H5. inv H2. cbn in H7.
+    inv H7; cbn in *; try invSome; invSome. simpl in H11; do 2 rewrite idsubst_is_id_exp in H11.
+    rename H11 into H5.
+    apply term_eval_both in H5 as T. destruct T as [res [l [Hres [D0 [D1 Hlia]]]]].
+    eapply term_step_term in H5. 2: eassumption. 2: auto.
+    clear D1. inv Hres.
+    - inv H5. eexists. eapply frame_indep_nil in D0. eapply step_term_term_plus.
+      eassumption. constructor. reflexivity. eassumption.
+    - inv H5.
+      + eapply frame_indep_nil in D0. eexists.
+        eapply step_term_term_plus. eassumption.
+        cbn in *. clear D0. eapply step_case_true. eassumption.
+      + inv H2; inv H11. simpl in H12. inv H12. inv H5. inv H10. 2: inv_val.
+        replace (map
+       (fun '(p, x0, y) =>
+        (p, x0.[upn (PatListScope p) idsubst],
+         y.[upn (PatListScope p) idsubst])) le) with le in H7.
+        replace (map (fun x0 : Exp => x0.[idsubst]) (map VVal lv)) with (map VVal lv) in H7.
+        2: {
+          clear. induction lv; auto. simpl. rewrite idsubst_is_id_val.
+          now rewrite IHlv at 1.
+        }
+        2: {
+          clear. induction le; auto. simpl. destruct a, p.
+          rewrite idsubst_upn, <-IHle.
+          now do 2 rewrite idsubst_is_id_exp.
+        }
+        destruct lv.
+        ** inv H7. inv H5. cbn in H11. cbn in H8. invSome.
+           eapply frame_indep_nil in D0. eexists.
+           eapply step_term_term_plus. eassumption.
+           eapply step_case_false. eassumption.
+        ** inv H7. inv H5. inv H12. eapply term_step_term in H6.
+           2: eapply params_eval_create. 2: { inv H. now inv H8. }
+           2: { reflexivity. }
+           simpl in H6.
+           eapply frame_indep_nil in D0. eexists.
+           eapply step_term_term_plus. eassumption.
+           eapply step_case_false. eassumption.
+(*   * simpl in H0. repeat deriv. (* receive is not evaluated at this level *)
+  * simpl in H0. repeat deriv. (* receive is not evaluated at this level *) *)
+Qed.
+*)
